src/Trace.v
@@ -368,6 +368,7 @@ Module Euf_Checker.
   | BBZextend (pos:int) (orig:clause_id) (res:_lit)
   | BBSextend (pos:int) (orig:clause_id) (res:_lit)
   | BBShl (pos:int) (orig1 orig2:clause_id) (res:_lit)
+  | BBShr (pos:int) (orig1 orig2:clause_id) (res:_lit)
   | RowEq (pos:int) (res: _lit)
   | RowNeq (pos:int) (cl: C.t)
   | Ext (pos:int) (res: _lit)
@@ -417,6 +418,7 @@ Module Euf_Checker.
       | BBZextend pos orig res => S.set_clause s pos (check_bbZextend t_atom t_form s orig res)
       | BBSextend pos orig res => S.set_clause s pos (check_bbSextend t_atom t_form s orig res)
       | BBShl pos orig1 orig2 res => S.set_clause s pos (check_bbShl t_atom t_form s orig1 orig2 res)
+      | BBShr pos orig1 orig2 res => S.set_clause s pos (check_bbShr t_atom t_form s orig1 orig2 res)
       | RowEq pos res => S.set_clause s pos (check_roweq t_form t_atom res)
       | RowNeq pos cl => S.set_clause s pos (check_rowneq t_form t_atom cl)
       | Ext pos res => S.set_clause s pos (check_ext t_form t_atom res)
@@ -440,7 +442,7 @@ Module Euf_Checker.
     |pos orig res|pos res|pos res|pos orig1 orig2 res|pos orig res|pos orig res
     |pos orig1 orig2 res|pos orig1 orig2 res
     |pos orig1 orig2 res|pos orig1 orig2 res|pos orig1 orig2 res|pos orig1 orig2 res
-    |pos cl |pos orig res |pos orig res |pos orig res | pos orig1 orig2 res |pos res|pos res 
+    |pos cl |pos orig res |pos orig res |pos orig res | pos orig1 orig2 res | pos orig1 orig2 res |pos res|pos res 
     |pos res |pos prem_id prem concl p]; simpl; try apply S.valid_set_clause; auto.
     - apply S.valid_set_resolve; auto.
     - apply S.valid_set_weaken; auto.
@@ -478,6 +480,7 @@ Module Euf_Checker.
     - apply valid_check_bbZextend; auto.
     - apply valid_check_bbSextend; auto.
     - apply valid_check_bbShl; auto.
+    - apply valid_check_bbShr; auto.
     - apply valid_check_roweq; auto.
     - apply valid_check_rowneq; auto.
     - apply valid_check_ext; auto.
